theories/iris/iris_wp_def.v
@@ -154,6 +154,20 @@ Definition mem_block `{!wasmG Σ} (n: N) (m: memory) :=
 Definition mem_block_at_pos `{!wasmG Σ} (n: N) (l:bytes) k :=
   ([∗ list] i ↦ b ∈ l, n ↦[wm][ (N.of_nat (N.to_nat k+i)) ] b)%I.
 
+Definition mem_equiv (m1 m2: memory): Prop :=
+  m1.(mem_max_opt) = m2.(mem_max_opt) /\
+  m1.(mem_data).(ml_data) = m2.(mem_data).(ml_data).
+
+Lemma mem_equiv_wmblock_rewrite (m1 m2: memory) n:
+  mem_equiv m1 m2 ->
+  (n ↦[wmblock] m1)%I ≡ (n ↦[wmblock] m2)%I.
+Proof.
+  unfold mem_equiv, mem_block.
+  destruct m1, m2.
+  destruct mem_data, mem_data0 => //=.
+  by move => [-> ->] => //.
+Qed.
+
 Definition tab_block `{!wasmG Σ} (n: N) (tab: tableinst) :=
   (([∗ list] i ↦ tabelem ∈ (tab.(table_data)), n ↦[wt][ (N.of_nat i) ] tabelem ) ∗
      (n ↪[wtsize] (tab_size tab)) ∗ (n ↪[wtlimit] (table_max_opt tab)))%I.
