theories/stdpp_aux.v
@@ -2,6 +2,123 @@ From mathcomp Require Import ssreflect eqtype seq ssrbool.
 From stdpp Require Import list fin_maps gmap.
 Require Import list_extra properties.
 
+(* Additional lemmas to reduce friction among stdpp/ssreflect/coq*)
+
+Ltac forward H Hname :=
+  lazymatch type of H with
+  | ?Hx -> _ => let Hp := fresh "Hp" in
+              assert Hx as Hp; last specialize (H Hp) as Hname end.
+
+(* automatically remembers a lookup result and make the hypothesis ready for destruct *)
+Ltac remember_lookup :=
+  match goal with
+  | |- context C [?m !! ?x = _] =>
+    let Hlookup := fresh "Hlookup" in
+    remember (m !! x) as lookup_res eqn: Hlookup; symmetry in Hlookup
+  end.
+
+(* resolving predicates related to maps and lookups in stdpp. *)
+Ltac resolve_finmap :=
+  repeat match goal with
+         | H: (list_to_map _) !! _ = Some _ |- _ =>
+           let H2 := fresh "H2" in 
+           apply elem_of_list_to_map in H as H2; clear H
+         | H: (list_to_map _) !! _ = None |- _ =>
+           let H2 := fresh "H2" in 
+           apply not_elem_of_list_to_map in H as H2; clear H
+         | H: _ ∈ fmap _ _ |- _ =>
+           let Heq := fresh "Heq" in
+           let Helem := fresh "Helem" in
+           apply elem_of_list_fmap in H; destruct H as [? [Heq Helem]]; subst; simpl in *
+         | H: ?x ∈ map_to_list _ |- _ =>
+           destruct x; apply elem_of_map_to_list in H
+         | H: _ ∈ imap _ _ |- _ =>
+           let Heq := fresh "Heq" in
+           let Helem := fresh "Helem" in
+           apply elem_of_lookup_imap in H; destruct H as [? [? [Heq Helem]]]
+         | H: (_, _) = (_, _) |- _ =>
+           inversion H; subst; clear H
+         | H: _ |- NoDup (fmap fst _) =>
+           apply NoDup_fmap_fst; intros; subst; simpl in *; try by []
+         | H: _ |- NoDup (map_to_list _) =>
+           apply NoDup_map_to_list; try by []
+         | H1: ?m !! ?x = _, H2: ?m !! ?x = _ |- _ =>
+           rewrite H2 in H1; subst; simpl in *; clear H2
+         | H: Some _ = Some _ |- _ =>
+           inversion H; subst; simpl in *; try by []
+         | H: _ |- (_, _) ∈ map_to_list _ =>
+           apply elem_of_map_to_list
+         | H: _ ∈ ?l |- _ =>
+           let Helem := fresh "Helem" in
+           try is_var l; apply elem_of_list_lookup in H; destruct H as [? Helem]
+         | _ => simpl in *; try by eauto
+         end.
+
+(* Turns out that this is surprisingly not a standard lemma in stdpp and non-trivial to prove. *)
+Lemma nodup_imap_inj1 {T X: Type} (l: list T) (f: nat -> T -> X):
+  (forall n1 n2 t1 t2, f n1 t1 = f n2 t2 -> n1 = n2) ->
+  NoDup (imap f l).
+Proof.
+  move: f.
+  induction l => //=; first by intros; apply NoDup_nil.
+  move => f HInj1. apply NoDup_cons. split.
+  - move => HContra. apply elem_of_lookup_imap in HContra.
+    destruct HContra as [i [y [Heq Helem]]].
+    by apply HInj1 in Heq.
+  - apply IHl. move => n1 n2 t1 t2 Heq.
+    simpl in Heq. apply HInj1 in Heq. lia.
+Qed.
+    
+Definition map_related {K: Type} {M: Type -> Type} {H0: forall A: Type, Lookup K A (M A)} {A: Type} (r: relation A) (m1 m2: M A) :=
+  forall (i: K) (x: A), m1 !! i = Some x -> exists y, m2 !! i = Some y /\ r x y.
+
+Lemma N_nat_bin n:
+  n = N.of_nat (ssrnat.nat_of_bin n).
+Proof.
+  destruct n => //=.
+  replace (ssrnat.nat_of_pos p) with (Pos.to_nat p); first by rewrite positive_nat_N.
+  induction p => //=.
+  - rewrite Pos2Nat.inj_xI.
+    f_equal.
+    rewrite IHp.
+    rewrite ssrnat.NatTrec.doubleE.
+    rewrite - ssrnat.mul2n.
+    by lias.
+  - rewrite Pos2Nat.inj_xO.
+    rewrite IHp.
+    rewrite ssrnat.NatTrec.doubleE.
+    rewrite - ssrnat.mul2n.
+    by lias.
+Qed.
+
+Lemma fold_left_preserve {A B: Type} (P: A -> Prop) (f: A -> B -> A) (l: list B) (acc: A) :
+  P acc ->
+  (forall (x:A) (act: B), P x -> P (f x act)) ->
+  P (fold_left f l acc).
+Proof.
+  rewrite -fold_left_rev_right.
+  revert acc.
+  induction l;simpl;auto.
+  intros acc Ha Hnext.
+  rewrite foldr_snoc /=. apply IHl =>//.
+  apply Hnext=>//.
+Qed.    
+
+Lemma nat_bin n:
+  ssrnat.nat_of_bin n = N.to_nat n.
+Proof.
+  rewrite -> (N_nat_bin n).
+  rewrite Nat2N.id.
+  by rewrite <- N_nat_bin.
+Qed.
+  
+Lemma take_all_alt {X: Type} (l: list X) n:
+  n = length l ->
+  take n l = l.
+Proof.
+  move => H. subst. by rewrite firstn_all.
+Qed.
+
 Lemma map_fmap {T1 T2: Type} (f: T1 -> T2) (l: list T1):
   map f l = fmap f l.
 Proof.
@@ -101,6 +218,118 @@ Proof.
     by rewrite repeat_length in Hlookup.
 Qed.
 
+Lemma seq_map_fmap {X Y: Type} (f: X -> Y) (l: list X):
+  seq.map f l = fmap f l.
+Proof.
+  by [].
+Qed.
+
+Lemma repeat_lookup_Some {X: Type} n (v: X) i res:
+  repeat v n !! i = Some res ->
+  res = v /\ i < n.
+Proof.
+  move => Hrlookup.
+  assert (i < length (repeat v n)); first by eapply lookup_lt_Some.
+
+  split; last by rewrite repeat_length in H.
+  assert (repeat v n !! i = Some v); first by apply repeat_lookup; rewrite repeat_length in H.
+  rewrite H0 in Hrlookup.
+  by inversion Hrlookup.
+Qed.
+
+Lemma zip_lookup_Some {T1 T2: Type} (l1 : list T1) (l2: list T2) i x1 x2:
+  length l1 = length l2 ->
+  l1 !! i = Some x1 ->
+  l2 !! i = Some x2 ->
+  (zip l1 l2) !! i = Some (x1, x2).
+Proof.
+  move : l2 i x1 x2.
+  induction l1; intros; destruct l2; destruct i => //=.
+  - simpl in *.
+    by inversion H0; inversion H1.
+  - simpl in *.
+    apply IHl1 => //.
+    by inversion H.
+Qed.
+
+Lemma zip_lookup_Some_inv {X Y: Type} (l1: list X) (l2: list Y) k v1 v2:
+  (zip l1 l2) !! k = Some (v1, v2) ->
+  l1 !! k = Some v1 /\ l2 !! k = Some v2.
+Proof.
+  move: l2 k v1 v2.
+  induction l1; intros; destruct l2; destruct k; simpl in * => //=.
+  - by inversion H.
+  - by apply IHl1.
+Qed.
+    
+Lemma list_to_map_zip_lookup {X Y: Type} (E: EqDecision X) (H: Countable X) (l1 : list X) (l2: list Y) (k: X) (v: Y) (m: gmap X Y):
+  NoDup l1 ->
+  length l1 = length l2 ->
+  (((list_to_map (zip l1 l2)): gmap X Y) !! k = Some v <->
+   (exists k', l1 !! k' = Some k /\ l2 !! k' = Some v)).
+Proof.
+  move => Hnd Hlen.
+  split; move => Hl.
+  { rewrite <- elem_of_list_to_map in Hl; last first.
+    { rewrite fst_zip => //; by lias. }
+    resolve_finmap.
+    exists x.
+    by apply zip_lookup_Some_inv in Helem.
+  }
+  destruct Hl as [k' [Hl1 Hl2]].
+  rewrite <- elem_of_list_to_map; last first.
+  { rewrite fst_zip => //; by lias. }
+  apply elem_of_list_lookup.
+  exists k'.
+  by apply zip_lookup_Some.
+Qed.
+  
+Lemma list_to_map_zip_insert {X Y: Type} (E: EqDecision X) (H: Countable X) (l1 : list X) (l2: list Y) (k: X) (k': nat) (v: Y) (m: gmap X Y):
+  NoDup l1 ->
+  m = list_to_map (zip l1 l2) ->
+  length l1 = length l2 ->
+  l1 !! k' = Some k ->
+  <[ k := v ]> m = list_to_map (zip l1 (<[ k' := v ]> l2)).
+Proof.
+  move => Hnd -> Hlen Hk.
+  apply map_eq.
+  move => i.
+  destruct (decide (i=k)); subst => //=.
+  - rewrite lookup_insert.
+    symmetry.
+    rewrite list_to_map_zip_lookup => //.
+    { exists k'.
+      split => //.
+      rewrite list_lookup_insert => //.
+      by apply lookup_lt_Some in Hk; lias.
+    }
+    { by rewrite insert_length. }
+  - rewrite lookup_insert_ne => //.
+    destruct (list_to_map (zip l1 _) !! i) eqn:Hli => /=.
+    { symmetry.
+      apply list_to_map_zip_lookup => //.
+      { by rewrite insert_length. }
+      { apply elem_of_list_to_map in Hli; last first.
+        { rewrite fst_zip => //; by lias. }
+        apply elem_of_list_lookup in Hli.
+        destruct Hli as [j Hli].
+        apply zip_lookup_Some_inv in Hli.
+        exists j.
+        rewrite list_lookup_insert_ne => //.
+        destruct Hli as [Hli _].
+        move => HContra; subst.
+        by rewrite Hk in Hli; inversion Hli.
+      }
+    }
+    {
+      resolve_finmap.
+      rewrite fst_zip in H2; last by lias.
+      rewrite not_elem_of_list_to_map_1 => //.
+      rewrite fst_zip => //.
+      by rewrite insert_length; lias.
+    }
+Qed.
+    
 Lemma fmap_fmap_lookup {T1 T2 T: Type} (f1: T1 -> T) (f2: T2 -> T) (l1: list T1) (l2: list T2):
   fmap f1 l1 = fmap f2 l2 ->
   forall i, fmap f1 (l1 !! i) = fmap f2 (l2 !! i).
@@ -119,3 +348,11 @@ Proof.
   - by apply lookup_lt_Some in Hl1; apply lookup_ge_None in Hl2; lias.
   - by apply lookup_lt_Some in Hl2; apply lookup_ge_None in Hl1; lias.
 Qed.
+
+Lemma skipn_is_drop_n {T: Type} (l: list T) n:
+  drop n l = seq.drop n l.
+Proof.
+  move: n.
+  by induction l; destruct n => //=.
+Qed.
+  
